final code

PL_final_proj_code.v
@@ -1,7 +1,8 @@
 (********************************************)
 (** Simple Toy Stack Language **)
 Require Import Coq.Strings.String.
-Require Import Coq.Strings.Ascii.
+(*Require Import Coq.Strings.Ascii.*)
+From Coq Require Import Arith.EqNat. Import Nat.
 Require Import String.
 Require Import List.
 Import ListNotations.
@@ -14,8 +15,8 @@ Inductive data : Type :=
   | num : nat -> data
   | bl : bool -> data.
 
-Definition state_ := total_map data.     (* define the state and empty state *)
-Definition empty_st := (t_empty (bl false)).
+Definition state := total_map nat.     (* define the state and empty state *)
+(*Definition empty_st := (t_empty (bl false)).*)
 
 (* example for how to use data types *)
 Definition eval_data (d : data) : data :=
@@ -24,181 +25,364 @@ Definition eval_data (d : data) : data :=
   | bl b => bl b
   end.
 
-(* data expressions are the numerical and boolean operations*)
-Inductive data_exp : Type :=
-  | NNum (d : data)
-  | NVar (x : string)
-  | NAdd (x y : data)
-  | NSub (x y : data)
-  | NMul (x y : data)
-  | NAnd (x y : data)
-  | NNot (d : data).
-
-Definition eval_exp (st : state_) (e : data_exp) : data :=
-  match e with
-  | NNum (num n) => num n
-  | NNum (bl b) => bl b
-  | NVar x => st x
-  | NAdd (num x) (num y) => num (x + y)
-  | NAdd (num x) (bl _) => num x
-  | NAdd (bl _) (num y) => num y
-  | NAdd (bl _) (bl _) => bl false
-  | NSub (num x) (num y) => num (x - y)
-  | NSub (num x) (bl _) => num x
-  | NSub (bl _) (num y) => num y
-  | NSub (bl _) (bl _) => bl false
-  | NMul (num x) (num y) => num (x * y)
-  | NMul (num x) (bl _) => num x
-  | NMul (bl _) (num y) => num y
-  | NMul (bl _) (bl _) => bl false
-  | NAnd (bl x) (bl y) => bl (andb x y)
-  | NAnd (bl x) (num y) => match x with
-      | true => num y
-      | false => bl false
-      end
-  | NAnd (num x) (bl y) => match y with
-      | true => num x
-      | false => bl false
-      end
-  | NAnd (num _) (num _) => bl false
-  | NNot (bl x) => bl (negb x)
-  | NNot (num _) => bl false
-  end.
-
 (* instructions are what programs are built from *)
 Inductive instr : Type :=
   | Push (d : data)
   | Load (x : string)
   | Asgn (x : string)
-  | DExp (de : data_exp).
+  | End
+  | NVal
+  | NAdd
+  | NSub
+  | NMul
+  | NEq
+  | NNeq
+  | NLe
+  | NGt
+  | NAnd
+  | NNot.
 
-(* evaluate a single instruction on a given stack and state *)
-Definition eval_instr (st : state_) (stack : list data) (i : instr) : list data :=
-  match i with
-  | Push d => d::stack
-  | Load x => (st x)::stack
-  | Asgn x => stack
-  | DExp de => match (de, stack) with
-      | (NNum _, dx::stack') => (eval_exp st (NNum dx))::stack
-      | (NVar x, stack) => (eval_exp st (NVar x))::stack
-      | (NAdd _ _, dx::dy::stack') => (eval_exp st (NAdd dx dy))::stack'
-      | (NSub _ _, dx::dy::stack') => (eval_exp st (NSub dx dy))::stack'
-      | (NMul _ _, dx::dy::stack') => (eval_exp st (NMul dx dy))::stack'
-      | (NAnd _ _, dx::dy::stack') => (eval_exp st (NAnd dx dy))::stack'
-      | (NNot _, dx::stack') => (eval_exp st (NNot dx))::stack'
-      | (_, []) => stack
-      | (_, [_]) => stack
+Definition eval_exp (st : state) (e : instr) (d1 d2 : data) : data :=
+  match (e, d1, d2) with
+  | (NVal, _, _) => d1
+  | (NAdd, (num x), (num y)) => num (x + y)
+  | (NAdd, (num x), (bl _)) => num x
+  | (NAdd, (bl _), (num y)) => num y
+  | (NAdd, (bl _), (bl _)) => bl false
+  | (NSub, (num x), (num y)) => num (x - y)
+  | (NSub, (num x), (bl _)) => num x
+  | (NSub, (bl _), (num y)) => num y
+  | (NSub, (bl _), (bl _)) => bl false
+  | (NMul, (num x), (num y)) => num (x * y)
+  | (NMul, (num x), (bl _)) => num x
+  | (NMul, (bl _), (num y)) => num y
+  | (NMul, (bl _), (bl _)) => bl false
+  | (NEq, (num x), (num y)) => bl (x =? y)
+  | (NEq, (bl true), (bl true)) => bl true
+  | (NEq, (bl false), (bl false)) => bl true
+  | (NEq, _, _) => bl false
+  | (NNeq, (num x), (num y)) => bl (negb (x =? y))
+  | (NNeq, (bl true), (bl true)) => bl false
+  | (NNeq, (bl false), (bl false)) => bl false
+  | (NNeq, _, _) => bl true
+  | (NLe, (num x), (num y)) => bl (x <=? y)
+  | (NLe, _, _) => bl false
+  | (NGt, (num x), (num y)) => bl (negb (x <=? y))
+  | (NGt, _, _) => bl false
+  | (NAnd, (bl x), (bl y)) => bl (andb x y)
+  | (NAnd, (bl x), (num y)) => match x with
+      | true => num y
+      | false => bl false
       end
+  | (NAnd, (num x), (bl y)) => match y with
+      | true => num x
+      | false => bl false
+      end
+  | (NAnd, (num x), (num _)) => num x (*bl false*)
+  | (NNot, (bl x), _) => bl (negb x)
+  | (NNot, (num _), _) => bl false
+  | _ => bl false
   end.
 
-(* evaluate entire program (list instr) on stack and state *)
-Fixpoint execute (st : state_) (stack : list data) (program : list instr) : (state_ * list data) :=
-  match program with
-  | (Push d)::p' => execute st (d::stack) p'
-  | (Load x)::p' => execute st ((st x)::stack) p'
-  | (Asgn x)::p' => match stack with
-      | d::stack' => let st' := t_update st x d in
-          execute st' stack' p'
-      | nil => execute st stack p'
+(* evaluate a single instruction on a given stack and state *)
+Definition eval_instr (st : state) (stack : list data) (i : instr) : (state * list data) :=
+  match i with
+  | Push d => (st, d::stack)
+  | Load x => (st, (num (st x))::stack)
+  | Asgn x => match stack with    (* PLACE HOLDER *)
+      | (num n)::stack' => let st' := t_update st x n in (st', stack')
+      | _::stack' => (st, stack')
+      | nil => (st, stack)
       end
-  | (DExp de)::p' => match (de, stack) with
-      | (NNum _, dx::stack') => execute st ((eval_exp st (NNum dx))::stack) p'
-      | (NVar x, stack) => execute st ((eval_exp st (NVar x))::stack) p'
-      | (NAdd _ _, dx::dy::stack') => execute st ((eval_exp st (NAdd dx dy))::stack') p'
-      | (NSub _ _, dx::dy::stack') => execute st ((eval_exp st (NSub dx dy))::stack') p'
-      | (NMul _ _, dx::dy::stack') => execute st ((eval_exp st (NMul dx dy))::stack') p'
-      | (NAnd _ _, dx::dy::stack') => execute st ((eval_exp st (NAnd dx dy))::stack') p'
-      | (NNot _, dx::stack') => execute st ((eval_exp st (NNot dx))::stack') p'
-      | (_, []) => (st, stack)
-      | (_, [_]) => (st, stack)
+  | End => match stack with 
+      | [] => (st, stack)
+      | _ => (st, stack)
       end
-  | _ => (st, stack)
+  | NVal => match stack with
+      | dx::stack' => (st, (eval_exp st NVal dx (bl false))::stack') (*dx::stack*)
+      | _ => (st, [])
+      end
+  | NAdd => match stack with
+      | dx::dy::stack' => (st, (eval_exp st NAdd dx dy)::stack')
+      | _ => (st, [])
+      end
+  | NSub => match stack with
+      | dx::dy::stack' => (st, (eval_exp st NSub dx dy)::stack')
+      | _ => (st, [])
+      end
+  | NMul => match stack with
+      | dx::dy::stack' => (st, (eval_exp st NMul dx dy)::stack')
+      | _ => (st, [])
+      end
+  | NEq => match stack with
+      | dx::dy::stack' => (st, (eval_exp st NEq dx dy)::stack')
+      | _ => (st, [])
+      end
+  | NNeq => match stack with
+      | dx::dy::stack' => (st, (eval_exp st NNeq dx dy)::stack')
+      | _ => (st, [])
+      end
+  | NLe => match stack with
+      | dx::dy::stack' => (st, (eval_exp st NLe dx dy)::stack')
+      | _ => (st, [])
+      end
+  | NGt => match stack with
+      | dx::dy::stack' => (st, (eval_exp st NGt dx dy)::stack')
+      | _ => (st, [])
+      end
+  | NAnd => match stack with
+      | dx::dy::stack' => (st, (eval_exp st NAnd dx dy)::stack')
+      | _ => (st, [])
+      end
+  | NNot => match stack with
+      | dx::stack' => (st, (eval_exp st NNot dx (bl false))::stack')
+      | _ => (st, [])
+      end
+  end.
   
+  
+
+(* evaluate entire program (list instr) on stack and state *)
+Fixpoint execute (st : state) (stack : list data) (program : list instr) : (state * list data) :=
+  match program with
+  | (Push d)::p' => let (st', stack') := eval_instr st stack (Push d) in execute st' stack' p'
+  | (Load x)::p' => let (st', stack') := eval_instr st stack (Load x) in execute st' stack' p'
+  | (Asgn x)::p' => let (st', stack') := eval_instr st stack (Asgn x) in execute st' stack' p'
+  | End::_ => eval_instr st stack End
+  | NVal::p' => let (st', stack') := eval_instr st stack NVal in execute st' stack' p'
+  | NAdd::p' => let (st', stack') := eval_instr st stack NAdd in execute st' stack' p'
+  | NSub::p' => let (st', stack') := eval_instr st stack NSub in execute st' stack' p'
+  | NMul::p' => let (st', stack') := eval_instr st stack NMul in execute st' stack' p'
+  | NEq::p' => let (st', stack') := eval_instr st stack NEq in execute st' stack' p'
+  | NNeq::p' => let (st', stack') := eval_instr st stack NNeq in execute st' stack' p'
+  | NLe::p' => let (st', stack') := eval_instr st stack NLe in execute st' stack' p'
+  | NGt::p' => let (st', stack') := eval_instr st stack NGt in execute st' stack' p'
+  | NAnd::p' => let (st', stack') := eval_instr st stack NAnd in execute st' stack' p'
+  | NNot::p' => let (st', stack') := eval_instr st stack NNot in execute st' stack' p'
+  | _ => (st, stack)
   end.
 
 Check execute.
-
-(* Notation so it's easier to write instructions *)
-(*Notation "':[' NSub ']:'" := (DExp (NSub (num 0) (num 0))) (at level 50).*)
-Notation "'~[' NNot ']~'" := (DExp (NNot (bl false))) (at level 50).
-Notation "':[' e ']:'" := (DExp (e (num 0) (num 0))) (at level 50).
-
 
 (*
   ----- Example execute -----
 *)
 Example execute1 :
      execute empty_st []
-       [Push (num 5); Push (num 1); Push (num 3); :[NSub]: ]
+       [Push (num 5); Push (num 1); Push (num 3); NSub; End]
    = (empty_st, [(num 2); (num 5)]).
-Proof. simpl. reflexivity. Qed. 
+Proof. reflexivity. Qed. 
 
-Definition init_state1 : state_ := t_update (t_empty (bl false)) "X" (num 3).
+Definition init_state1 : state := t_update (empty_st) "X" 3.
 
 Example execute2 :
      execute init_state1 [(num 3); (num 4)]
-       [Push (num 4); Load "X"; :[NMul]:; :[NAdd]:]
+       [Push (num 4); Load "X"; NMul; NAdd; End]
    = (init_state1, [(num 15); (num 4)]).
 Proof. simpl. reflexivity. Qed.
 
-Definition init_state2 : state_ := t_update (t_empty (bl false)) "X" (bl true).
+Definition init_state2 : state := t_update (empty_st) "X" 1.
 
 Example execute3 :
      execute init_state2 [(bl true); (num 4); (bl false)]
-       [:[NAnd]:; Load "X"; :[NAnd]:]
-   = (init_state2, [(num 4); (bl false)]).
+       [NAnd; Load "X"; NAnd; End]
+   = (init_state2, [(num 1); (bl false)]).
 Proof. simpl. reflexivity. Qed.
-
-
 (* Compiling IMP to low-level *)
 
+(*--[  Compile arithmetic expressions into list of low-level instructions  ]--*)
 Fixpoint compile_aexp (a : aexp) : list instr :=
   match a with
-  | ANum n => [Push (num n)]
+  | ANum n => ([Push (num n)])
   | AId x => [Load x]
-  | APlus a1 a2 => compile_aexp a1 ++ compile_aexp a2 ++ [:[NAdd]:]
-  | AMinus a1 a2 => compile_aexp a1 ++ compile_aexp a2 ++ [:[NSub]:]
-  | AMult a1 a2 => compile_aexp a1 ++ compile_aexp a2 ++ [:[NMul]:]
+  | APlus a1 a2 => compile_aexp a1 ++ compile_aexp a2 ++ [NAdd]
+  | AMinus a1 a2 => compile_aexp a1 ++ compile_aexp a2 ++ [NSub]
+  | AMult a1 a2 => compile_aexp a1 ++ compile_aexp a2 ++ [NMul]
   end.
+
+Check compile_aexp.
+
+(*--[  Compile boolean expressions into list of low-level instructions  ]--*)
 Fixpoint compile_bexp (b : bexp) : list instr :=
   match b with
   | BTrue => [Push (bl true)]
   | BFalse => [Push (bl false)]
-  | BEq a1 a2 => compile_aexp a1 ++ compile_aexp a2 ++ [:[NAnd]:]
-  | BNeq a1 a2 => compile_aexp a1 ++ compile_aexp a2 ++ [:[NAnd]:]
-  | BLe a1 a2 => compile_aexp a1 ++ compile_aexp a2 ++ [:[NAnd]:]
-  | BGt a1 a2 => compile_aexp a1 ++ compile_aexp a2 ++ [:[NAnd]:]
-  | BNot b1 => compile_bexp b1 ++ [~[NNot]~]
-  | BAnd b1 b2 => compile_bexp b1 ++ compile_bexp b2 ++ [:[NAnd]:]
+  | BEq a1 a2 => compile_aexp a1 ++ compile_aexp a2 ++ [NEq]
+  | BNeq a1 a2 => compile_aexp a1 ++ compile_aexp a2 ++ [NNeq]
+  | BLe a1 a2 => compile_aexp a1 ++ compile_aexp a2 ++ [NLe]
+  | BGt a1 a2 => compile_aexp a1 ++ compile_aexp a2 ++ [NGt]
+  | BNot b1 => compile_bexp b1 ++ [NNot]
+  | BAnd b1 b2 => compile_bexp b1 ++ compile_bexp b2 ++ [NAnd]
   end.
 
 Check compile_bexp.
 
 Fixpoint compile (c : com) : list instr :=
   match c with
-  | CSkip => []
   | CAsgn x y => compile_aexp y ++ [Asgn x]
   | CSeq c1 c2 => compile c1 ++ compile c2
-  | CIf b c1 c2 =>
+  | CIf b c1 c2 =>                    (* <--- PLACE HOLDER *)
       let com_b := compile_bexp b in
       let com_bn := compile_bexp (BNot b) in
       let com_c1 := compile c1 in
       let com_c2 := compile c2 in
-      com_b ++ com_c1 ++ [:[NAnd]:] ++ com_bn ++ com_c2 ++ [:[NAnd]:]
-  | CWhile x y =>
+      com_b ++ com_c1 ++ [NAnd] ++ com_bn ++ com_c2 ++ [NAnd]
+  | CWhile x y =>                     (* <--- PLACE HOLDER *)
       let com_x := compile_bexp x in
       let com_y := compile y in
       com_x ++ com_y
+  | _ => []
   end.
 
-Check compile.
-
-Theorem compile_aexp_correct : forall (a : aexp) (st_ : state_) (st : state),
-  execute st_ [] (compile_aexp a) = (st_, [num (aeval st a)]).
+(*
+******** Proofs for various small things: ********
+*)
+Lemma execute_empty_stack :
+  forall st p,
+    execute st [] p = execute st [] p.
 Proof.
-  intros. 
+  simpl.  intros. induction p; reflexivity.
+Qed.
+
+Lemma ev_exec_push : forall st stack' i d1 d2,
+  execute st stack' ([Push d1]++[Push d2]++[i]) = eval_instr st ([d2]++[d1]++stack') i.
+Proof.
+  intros. induction i; try reflexivity. simpl. destruct d2; reflexivity.
+Qed.
+Lemma ev_exec_load : forall st stack' i x1 x2,
+  execute st stack' ([Load x1]++[Load x2]++[i]) = eval_instr st ([num (st x2)]++[num (st x1)]++stack') i.
+Proof.
+  intros. induction i; try reflexivity.
+Qed.
+Lemma ev_exec_pl : forall st stack' i d1 x2,
+  execute st stack' ([Push d1]++[Load x2]++[i]) = eval_instr st ([num (st x2)]++[d1]++stack') i.
+Proof.
+  intros. induction i; try reflexivity.
+Qed.
+Lemma ev_exec_lp : forall st stack' i x1 d2,
+  execute st stack' ([Load x1]++[Push d2]++[i]) = eval_instr st ([d2]++[num (st x1)]++stack') i.
+Proof.
+  intros. induction i; try reflexivity. simpl. destruct d2; reflexivity.
+Qed.
+
+Lemma execute_empty_program :
+  forall st stack p',
+    (st, stack) = execute st stack ([End]++p').
+Proof.
+  simpl. intros. induction stack; reflexivity.
+Qed.
+
+Lemma eval_end : forall st stack,
+  eval_instr st stack End = (st, stack).
+Proof.
+  intros. induction stack; try reflexivity.
+Qed.
+
+Lemma exec_end_ev : forall st stack p,
+  execute st stack ([End]++p) = eval_instr st stack End.
+Proof.
+  intros. simpl. reflexivity.
+Qed.
+
+Lemma exec_end : forall st stack p,
+  execute st stack ([End]++p) = (st, stack).
+Proof. 
+  intros. rewrite exec_end_ev. rewrite eval_end. easy.
+Qed.
+
+Definition is_end i : bool :=
+  match i with
+  | End => true
+  | _ => false
+  end.
+
+Lemma execute_i_p : forall st stack (i : instr) (p : list instr),
+  execute st stack ([i] ++ p) = (if (is_end i) then
+  eval_instr st stack i
+  else
+  let (st', stack') := eval_instr st stack i in
+  execute st' stack' p).
+Proof.
+  intros. induction i eqn:Ei; try reflexivity.
+Qed.
+
+Lemma p_assoc : forall (i : instr) (p1 p2 : list instr),
+  ((i :: p1) ++ p2) = [i]++p1++p2.
+Proof.
+  intros. rewrite <- app_comm_cons. reflexivity.
+Qed.
+
+Lemma stack_i_eq : forall (i : instr) (p : list instr),
+  ([i] ++ p) = (i::p).
+Proof.
+  intros. reflexivity.
+Qed.
+
+Lemma execute_app : forall st stack p1 p2,
+  execute st stack (p1 ++ p2) = 
+  let (st', stack') := execute st stack p1 in
+  execute st' stack' p2.
+Proof.
+  intros st stack p1 p2. generalize dependent stack. induction p1 as [| i p1' IH].
+  - reflexivity.
+  - rewrite -> p_assoc. intros. rewrite execute_i_p. 
+    rewrite <- stack_i_eq. rewrite execute_i_p. 
+    destruct i; simpl.
+    + . destruct d; simpl.
+      -- unfold execute.
+     apply IH.  generalize p2. rewrite <- IH. 
+  - rewrite -> p_assoc. rewrite -> execute_i_p.
+  Admitted.
+
+Theorem add_0_r : forall n:nat, n + 0 = n.
+Proof. intros n. 
+  induction n as [| n' IH].
+  * simpl. reflexivity.
+  * simpl. rewrite IH. reflexivity.
+Qed.
+Theorem add_comm : forall n m : nat,
+  n + m = m + n.
+Proof. intros n m.
+  induction n as [| n' IHn].
+  { simpl. 
+    rewrite add_0_r.
+    reflexivity. }
+  { simpl. 
+    rewrite IHn.
+    trivial. }
+Qed.
+    
+(*
+******** Proofs for compiling: ********
+*)
+(*--[  Prove compile_aexp  ]--*)
+Theorem compile_aexp_correct : forall st stack a,
+  execute st stack (compile_aexp a) = (st, [num (aeval st a)] ++ stack).
+Proof.
+  intros. generalize dependent stack. induction a; simpl; try reflexivity.
+  - rewrite execute_i_p.
+  - destruct a1; destruct a2; simpl; try (unfold eval_exp; rewrite add_comm; reflexivity).
+    + sim
+    + unfold eval_exp.
+   
+   - reflexivity.
+   - reflexivity. 
+   - unfold compile_aexp. rewrite IHa2.
 Admitted.
 
+
+(*--[  Prove compile_bexp  ]--*)
+(* - prove correct for just one instruction: *)
+Lemma compile_bexp_correct : forall st be,
+  execute st [] (compile_bexp be) = (st, [bl (beval st be)]).
+Proof.
+  intros. induction be; try reflexivity.
+  - simpl. destruct a1.
+    * Admitted.
+
+
+(*--[  Prove compile  ]--*)
+(* - prove correct for just one instruction: *)
 Theorem compile_correct : forall (c : com) (st st' : state) (st_ st'_ : state_),
   ceval c st st' -> execute st_ [] (compile c) = (st'_, []).
 Proof.
@@ -206,72 +390,6 @@ Proof.
   - unfold compile. admit.
   - admit.
 Admitted.
-
-(* Test compilation: *)
-Definition X : string := "X".
-Definition Y : string := "Y".
-Definition Z : string := "Z".
-
-(* 
-  Make IMP program and compile it: 
-   - Example 1 *)
-Definition ex1_program : com :=
-  CSeq (CAsgn Z (ANum 2)) (CAsgn X (ANum 6)).
-
-Definition ex1_compiled := compile ex1_program.
-Compute ex1_compiled.
-
-Definition final_state_and_stack := execute empty_st [] ex1_compiled.
-Definition final_state : state_ := fst final_state_and_stack.
-Definition final_stack : list data := snd final_state_and_stack.
-Compute final_state Z.
-Definition final_state_z_ll := final_state Z.
-
-Definition empty_st2 := (_ !-> 0).
-Compute ceval ex1_program empty_st2.
-
-
-(* Bisimilation Theorem *)
-Theorem bisim1 : forall st',
-    (ceval (CAsgn Z (ANum 2)) empty_st2 st') ->
-    st' Z = 2.
-Proof.
-  intros. (*apply E_Asgn in H.*)
-Admitted.
-
-Theorem bisim2 : forall st st',
-    (ceval (CSeq (CAsgn Z (ANum 2)) (CAsgn X (ANum 6))) st st') ->
-    num (st' Z) = final_state Z.
-Proof.
-Admitted.
-(*
-  apply CAsgn.
-  inversion Hceval; subst.
-*)
-
-(* Check against execution of Imp directly: *)
-Definition ex2_program : com :=
-  CIf (BAnd (BTrue) (BTrue)) 
-    (CAsgn "Z" (AMult (APlus (AId "X") (AId "Y")) (ANum 2)))
-    (CAsgn "Z" (ANum 0)).
-
-Definition ex2_compiled := compile ex1_program.
-
-Compute ex2_compiled.
-
-Definition init_state_ex2 : state := t_update (t_update (t_empty (bl false)) "X" (num 5)) "Y" (num 3).
-
-Compute execute init_state_ex2 [] ex1_compiled.
-
-Example compile2 :
-     execute empty_st []
-       [Push (num 5); Push (num 1); Push (num 3); :[NSub]: ]
-   = [(num 2); (num 5)].
-(* FILL IN HERE *)
-Proof. simpl. reflexivity. Qed. 
-
-
-
 
 
 
